single step semantics

SIL-Parallel/SIL_Star.thy
@@ -4,37 +4,18 @@ section "SIL Logic"
 
 subsection "SIL Logic for Partial Correctness"
 
-theory SIL imports Big_Step begin
+theory SIL_Star imports Small_Step SIL_Single_Step begin
 
-type_synonym assn = "state \<Rightarrow> bool"
-
-datatype post =
-    OK assn
-    | ER assn
-
-fun post_assn :: "post \<Rightarrow> assn" where
-  "post_assn (OK Q) = Q"
-| "post_assn (ER Q) = Q"
-
-fun post_ok :: "post \<Rightarrow> bool" where
-  "post_ok (OK Q) = True"
-| "post_ok (ER Q) = False"
-
-
-definition SIL_valid ::
+definition SIL_Star_Valid ::
   "assn \<Rightarrow> com \<Rightarrow> post \<Rightarrow> bool" (\<open>\<Turnstile> (\<langle>(1_)\<rangle>/ (_)/  \<langle>(1_)\<rangle>)\<close> 50)
 where
 "\<Turnstile> \<langle>P\<rangle> c \<langle>R\<rangle> \<equiv>
   (case R of
-      OK Q \<Rightarrow> (\<forall>s. P s \<longrightarrow> (\<exists>t. (c,s) \<Down> (t,True) \<and> Q t))
-    | ER Q \<Rightarrow> (\<forall>s. P s \<longrightarrow> (\<exists>t. (c,s) \<Down> (t,False) \<and> Q t)))"
-
-abbreviation state_subst :: "state \<Rightarrow> aexp \<Rightarrow> vname \<Rightarrow> state"
-  (\<open>_[_'/_]\<close> [1000,0,0] 999)
-where "s[a/x] == s(x := aval a s)"
+      OK Q \<Rightarrow> (\<forall>s. P s \<longrightarrow> (\<exists>t. (c, sOK s) \<rightarrow>* (SKIP, sOK t) \<and> Q t))
+    | ER Q \<Rightarrow> (\<forall>s. P s \<longrightarrow> (\<exists>t. (c, sOK s) \<rightarrow>* (SKIP, sER t) \<and> Q t)))"
 
 inductive
-  SIL :: "assn \<Rightarrow> com \<Rightarrow> post \<Rightarrow> bool" (\<open>\<turnstile> (\<langle>(1_)\<rangle>/ (_)/  \<langle>(1_)\<rangle>)\<close> 50)
+  SIL_Star :: "assn \<Rightarrow> com \<Rightarrow> post \<Rightarrow> bool" (\<open>\<turnstile> (\<langle>(1_)\<rangle>/ (_)/  \<langle>(1_)\<rangle>)\<close> 50)
 where
 tSkip: "\<turnstile> \<langle>P\<rangle> SKIP \<langle>OK P\<rangle>"  |
 
@@ -89,39 +70,58 @@ tWhileER: "
 \<Longrightarrow> 
   \<turnstile> \<langle>\<lambda>s. \<exists>n. Q (Suc n) s\<rangle>  WHILE b DO c \<langle>ER (Q 0)\<rangle>" |
 
-conseqOK: "\<lbrakk> \<forall>s. P' s \<longrightarrow> P s;  \<turnstile> \<langle>P\<rangle> c \<langle>OK Q\<rangle>;  \<forall>s. Q s \<longrightarrow> Q' s \<rbrakk>
+tConseqOK: "\<lbrakk> \<forall>s. P' s \<longrightarrow> P s;  \<turnstile> \<langle>P\<rangle> c \<langle>OK Q\<rangle>;  \<forall>s. Q s \<longrightarrow> Q' s \<rbrakk>
         \<Longrightarrow> \<turnstile> \<langle>P'\<rangle> c \<langle>OK Q'\<rangle>" |
 
-conseqER: "\<lbrakk> \<forall>s. P' s \<longrightarrow> P s;  \<turnstile> \<langle>P\<rangle> c \<langle>ER Q\<rangle>;  \<forall>s. Q s \<longrightarrow> Q' s \<rbrakk>
+tConseqER: "\<lbrakk> \<forall>s. P' s \<longrightarrow> P s;  \<turnstile> \<langle>P\<rangle> c \<langle>ER Q\<rangle>;  \<forall>s. Q s \<longrightarrow> Q' s \<rbrakk>
         \<Longrightarrow> \<turnstile> \<langle>P'\<rangle> c \<langle>ER Q'\<rangle>" |
 
-false_pre: "\<turnstile> \<langle>\<lambda>s. False\<rangle> c \<langle>Q\<rangle>" |
+tFalsePre: "\<turnstile> \<langle>\<lambda>s. False\<rangle> c \<langle>Q\<rangle>" |
 
-disjunction:  "\<lbrakk> \<turnstile> \<langle>P\<rangle> c \<langle>Q\<rangle>; \<turnstile> \<langle>R\<rangle> c \<langle>Q\<rangle> \<rbrakk> 
-        \<Longrightarrow> \<turnstile> \<langle>\<lambda>s. (P s \<or> R s)\<rangle> c \<langle>Q\<rangle>"
+tDisjunction:  "\<lbrakk> \<turnstile> \<langle>P\<rangle> c \<langle>Q\<rangle>; \<turnstile> \<langle>R\<rangle> c \<langle>Q\<rangle> \<rbrakk> 
+        \<Longrightarrow> \<turnstile> \<langle>\<lambda>s. (P s \<or> R s)\<rangle> c \<langle>Q\<rangle>" |
+
+tParallelL: "\<lbrakk> \<turnstile> \<langle>P\<rangle> c\<^sub>1 \<leadsto> c\<^sub>1'  \<langle>OK P'\<rangle>; \<turnstile> \<langle>P'\<rangle> c\<^sub>1'||c\<^sub>2 \<langle>Q\<rangle> \<rbrakk>
+        \<Longrightarrow> \<turnstile> \<langle>P\<rangle> c\<^sub>1||c\<^sub>2 \<langle>Q\<rangle>" |
+
+tParallelR: "\<lbrakk> \<turnstile> \<langle>P\<rangle> c\<^sub>2 \<leadsto> c\<^sub>2'  \<langle>OK P'\<rangle>; \<turnstile> \<langle>P'\<rangle> c\<^sub>1||c\<^sub>2' \<langle>Q\<rangle> \<rbrakk>
+        \<Longrightarrow> \<turnstile> \<langle>P\<rangle> c\<^sub>1||c\<^sub>2 \<langle>Q\<rangle>" |
+
+tParallelERL: "\<lbrakk> \<turnstile> \<langle>P\<rangle> c\<^sub>1 \<leadsto> c\<^sub>1'  \<langle>ER Q\<rangle>\<rbrakk>
+        \<Longrightarrow> \<turnstile> \<langle>P\<rangle> c\<^sub>1||c\<^sub>2 \<langle>ER Q\<rangle>" |
+
+tParallelERR: "\<lbrakk> \<turnstile> \<langle>P\<rangle> c\<^sub>2 \<leadsto> c\<^sub>2'  \<langle>ER Q\<rangle>\<rbrakk>
+        \<Longrightarrow> \<turnstile> \<langle>P\<rangle> c\<^sub>1||c\<^sub>2 \<langle>ER Q\<rangle>" |
+
+tParallelSkipL: "\<lbrakk> \<turnstile> \<langle>P\<rangle> c\<^sub>2  \<langle>Q\<rangle> \<rbrakk>
+        \<Longrightarrow> \<turnstile> \<langle>P\<rangle> SKIP||c\<^sub>2 \<langle>Q\<rangle>" |
+
+tParallelSkipR: "\<lbrakk> \<turnstile> \<langle>P\<rangle> c\<^sub>1  \<langle>Q\<rangle> \<rbrakk>
+        \<Longrightarrow> \<turnstile> \<langle>P\<rangle> c\<^sub>1||SKIP \<langle>Q\<rangle>"
+
 
 lemmas [simp] = SIL.tSkip SIL.tAssign SIL.tSeqOK tIf
 lemmas [intro!] = SIL.tSkip SIL.tAssign SIL.tSeqOK SIL.tIf
 
 lemma strengthen_pre:
   "\<lbrakk> \<forall>s. P' s \<longrightarrow> P s;  \<turnstile> \<langle>P\<rangle> c \<langle>R\<rangle> \<rbrakk> \<Longrightarrow> \<turnstile> \<langle>P'\<rangle> c \<langle>R\<rangle>"
-  by (smt (verit, ccfv_SIG) conseqER conseqOK post.exhaust)
+  by (smt (verit, ccfv_SIG) tConseqER tConseqOK post.exhaust)
 
 lemma strengthen_pre_ok:
   "\<lbrakk> \<forall>s. P' s \<longrightarrow> P s;  \<turnstile> \<langle>P\<rangle> c \<langle>OK Q\<rangle> \<rbrakk> \<Longrightarrow> \<turnstile> \<langle>P'\<rangle> c \<langle>OK Q\<rangle>"
-  by (simp add: conseqOK)
+  by (simp add: tConseqOK)
 
 lemma strengthen_pre_er:
   "\<lbrakk> \<forall>s. P' s \<longrightarrow> P s;  \<turnstile> \<langle>P\<rangle> c \<langle>ER Q\<rangle> \<rbrakk> \<Longrightarrow> \<turnstile> \<langle>P'\<rangle> c \<langle>ER Q\<rangle>"
-  by (simp add: conseqER)
+  by (simp add: tConseqER)
 
 lemma weaken_post_ok:
   "\<lbrakk> \<turnstile> \<langle>P\<rangle> c \<langle>OK Q\<rangle>;  \<forall>s. Q s \<longrightarrow> Q' s \<rbrakk> \<Longrightarrow>  \<turnstile> \<langle>P\<rangle> c \<langle>OK Q'\<rangle>"
-  using conseqOK by blast
+  using tConseqOK by blast
 
 lemma weaken_post_er:
   "\<lbrakk> \<turnstile> \<langle>P\<rangle> c \<langle>ER Q\<rangle>;  \<forall>s. Q s \<longrightarrow> Q' s \<rbrakk> \<Longrightarrow>  \<turnstile> \<langle>P\<rangle> c \<langle>ER Q'\<rangle>"
-  using conseqER by blast
+  using tConseqER by blast
 
 text\<open>The assignment and While rule are awkward to use in actual proofs
 because their pre and postcondition are of a very special form and the actual
@@ -129,6 +129,6 @@ goal would have to match this form exactly. Therefore we derive two variants
 with arbitrary pre and postconditions.\<close>
 
 lemma Assign': "\<forall>s. P s \<longrightarrow> Q(s[a/x]) \<Longrightarrow> \<turnstile> \<langle>P\<rangle> x ::= a \<langle>OK Q\<rangle>"
-  by (metis (lifting) conseqOK tAssign)
+  by (metis (lifting) tConseqOK tAssign)
 
 end
