SIL-Parallel/SIL_Single_Step.thy
@@ -1,0 +1,95 @@
+(* Author: Tobias Nipkow *)
+
+section "SIL Logic"
+
+subsection "SIL Logic for Partial Correctness"
+
+theory SIL_Single_Step imports Small_Step begin
+
+type_synonym assn = "state \<Rightarrow> bool"
+
+datatype post =
+    OK assn
+    | ER assn
+
+fun post_assn :: "post \<Rightarrow> assn" where
+  "post_assn (OK Q) = Q"
+| "post_assn (ER Q) = Q"
+
+fun post_ok :: "post \<Rightarrow> bool" where
+  "post_ok (OK Q) = True"
+| "post_ok (ER Q) = False"
+
+definition SIL_Single_Step_Valid ::
+  "assn \<Rightarrow> com \<Rightarrow> com \<Rightarrow> post \<Rightarrow> bool" (\<open>\<Turnstile> (\<langle>(1_)\<rangle>/ (_)/ \<leadsto> (_)/ \<langle>(1_)\<rangle>)\<close> 50)
+where
+"\<Turnstile> \<langle>P\<rangle> c1 \<leadsto> c2 \<langle>R\<rangle> \<equiv>
+      (case R of
+      OK Q \<Rightarrow> (\<forall>s. P s \<longrightarrow> (\<exists>s'. (c1,sOK s) \<rightarrow> (c2,sOK s') \<and> Q s'))
+    | ER Q \<Rightarrow> (\<forall>s. P s \<longrightarrow> (\<exists>s'. (c1,sOK s) \<rightarrow> (c2,sER s') \<and> Q s')))"
+
+
+abbreviation state_subst :: "state \<Rightarrow> aexp \<Rightarrow> vname \<Rightarrow> state"
+  (\<open>_[_'/_]\<close> [1000,0,0] 999)
+where "s[a/x] == s(x := aval a s)"
+
+inductive
+  SIL_Single_Step :: "assn \<Rightarrow> com \<Rightarrow> com \<Rightarrow> post \<Rightarrow> bool" (\<open>\<turnstile> (\<langle>(1_)\<rangle>/ (_)/ \<leadsto> (_)/ \<langle>(1_)\<rangle>)\<close> 50)
+where
+sAbort: "\<turnstile> \<langle>P\<rangle> ABORT \<leadsto> SKIP \<langle>ER P\<rangle>"  |
+
+sAssign:  "\<turnstile> \<langle>\<lambda>s. P(s[a/x])\<rangle> x::=a \<leadsto> SKIP \<langle>OK P\<rangle>"  |
+
+sAssignNDOK:  "\<turnstile> \<langle>\<lambda>s. (\<exists>v \<in> vals. P(s(x := aval v s)))\<rangle> x::= ND vals \<leadsto> SKIP \<langle>OK P\<rangle>"  |
+
+sAssignNDEmpty:  "\<turnstile> \<langle>P\<rangle> x ::= ND {} \<leadsto> ABORT \<langle>OK P\<rangle>"  |
+
+sSeq: "\<lbrakk> \<turnstile> \<langle>P\<rangle> c\<^sub>1 \<leadsto> c\<^sub>1' \<langle>R\<rangle>\<rbrakk>
+      \<Longrightarrow> \<turnstile> \<langle>P\<rangle> c\<^sub>1;;c\<^sub>2 \<leadsto> c\<^sub>1';;c\<^sub>2 \<langle>R\<rangle>"  |
+
+sSeqSkip: "\<turnstile> \<langle>P\<rangle> SKIP;;c\<^sub>2 \<leadsto> c\<^sub>2 \<langle>OK P\<rangle>"  |
+
+sIfTrue: "\<forall>s. P s \<longrightarrow> bval b s \<Longrightarrow> \<turnstile> \<langle>P\<rangle> IF b THEN c\<^sub>1 ELSE c\<^sub>2 \<leadsto> c\<^sub>1  \<langle>OK P\<rangle>"  |
+sIfFalse: "\<forall>s. P s \<longrightarrow> \<not>bval b s \<Longrightarrow> \<turnstile> \<langle>P\<rangle> IF b THEN c\<^sub>1 ELSE c\<^sub>2 \<leadsto> c\<^sub>2  \<langle>OK P\<rangle>"  |
+
+sSelectND: "\<lbrakk>(b,c) \<in> set bs; bval b s\<rbrakk>
+   \<Longrightarrow> \<turnstile> \<langle>\<lambda>s. P s \<and> bval b s\<rangle> SELECT bs \<leadsto> c \<langle>OK P\<rangle>" |
+
+sSelectNDNP: (* No Path *)
+"\<lbrakk>\<forall>s. P s \<longrightarrow> (\<forall>(b, c) \<in> set bs. \<not>bval b s)\<rbrakk>
+   \<Longrightarrow> \<turnstile> \<langle>P\<rangle> SELECT bs \<leadsto> ABORT \<langle>OK P\<rangle>" |
+
+sWhile: "\<turnstile> \<langle>P\<rangle> WHILE b DO c \<leadsto> IF b THEN c;;WHILE b DO c ELSE SKIP \<langle>OK P\<rangle>" |
+
+sConseqOK: "\<lbrakk> \<forall>s. P' s \<longrightarrow> P s;  \<turnstile> \<langle>P\<rangle> c \<leadsto> c' \<langle>OK Q\<rangle>;  \<forall>s. Q s \<longrightarrow> Q' s \<rbrakk>
+        \<Longrightarrow> \<turnstile> \<langle>P'\<rangle> c \<leadsto> c' \<langle>OK Q'\<rangle>" |
+
+sConseqER: "\<lbrakk> \<forall>s. P' s \<longrightarrow> P s;  \<turnstile> \<langle>P\<rangle> c \<leadsto> c' \<langle>ER Q\<rangle>;  \<forall>s. Q s \<longrightarrow> Q' s \<rbrakk>
+        \<Longrightarrow> \<turnstile> \<langle>P'\<rangle> c \<leadsto> c' \<langle>ER Q'\<rangle>" |
+
+sFalsePre: "\<turnstile> \<langle>\<lambda>s. False\<rangle> c \<leadsto> c' \<langle>Q\<rangle>" |
+
+sDisjunction:  "\<lbrakk> \<turnstile> \<langle>P\<rangle> c \<leadsto> c' \<langle>Q\<rangle>; \<turnstile> \<langle>R\<rangle> c \<leadsto> c' \<langle>Q\<rangle> \<rbrakk> 
+        \<Longrightarrow> \<turnstile> \<langle>\<lambda>s. (P s \<or> R s)\<rangle> c \<leadsto> c' \<langle>Q\<rangle>"
+
+lemma strengthen_pre:
+  "\<lbrakk> \<forall>s. P' s \<longrightarrow> P s;  \<turnstile> \<langle>P\<rangle> c \<leadsto> c' \<langle>R\<rangle> \<rbrakk> \<Longrightarrow> \<turnstile> \<langle>P'\<rangle> c \<leadsto> c' \<langle>R\<rangle>"
+  by (smt (verit, ccfv_SIG) post_assn.elims sConseqER sConseqOK)
+
+lemma weaken_post_ok:
+  "\<lbrakk> \<turnstile> \<langle>P\<rangle> c \<leadsto> c' \<langle>OK Q\<rangle>;  \<forall>s. Q s \<longrightarrow> Q' s \<rbrakk> \<Longrightarrow>  \<turnstile> \<langle>P\<rangle> c \<leadsto> c' \<langle>OK Q'\<rangle>"
+  using sConseqOK by blast
+
+lemma weaken_post_er:
+  "\<lbrakk> \<turnstile> \<langle>P\<rangle> c \<leadsto> c' \<langle>ER Q\<rangle>;  \<forall>s. Q s \<longrightarrow> Q' s \<rbrakk> \<Longrightarrow>  \<turnstile> \<langle>P\<rangle> c \<leadsto> c' \<langle>ER Q'\<rangle>"
+  using sConseqER by blast
+
+text\<open>The assignment and While rule are awkward to use in actual proofs
+because their pre and postcondition are of a very special form and the actual
+goal would have to match this form exactly. Therefore we derive two variants
+with arbitrary pre and postconditions.\<close>
+
+lemma Assign': "\<forall>s. P s \<longrightarrow> Q(s[a/x]) \<Longrightarrow> \<turnstile> \<langle>P\<rangle> x ::= a \<leadsto> SKIP \<langle>OK Q\<rangle>"
+  by (simp add: sAssign strengthen_pre)
+
+end
