SIL-Parallel/SIL_Single_Step_Sound.thy
@@ -1,0 +1,38 @@
+subsection \<open>Soundness and Completeness\<close>
+
+theory SIL_Single_Step_Sound
+imports SIL_Single_Step
+begin
+
+subsubsection "Soundness"
+
+lemma sil_single_step_sound: 
+  "\<turnstile> \<langle>P\<rangle>c \<leadsto> c'\<langle>R\<rangle>  \<Longrightarrow>  \<Turnstile> \<langle>P\<rangle>c \<leadsto> c'\<langle>R\<rangle>"
+  unfolding SIL_Single_Step_Valid_def
+  apply (induction rule:SIL_Single_Step.induct; fastforce?)
+         apply (case_tac R)
+         apply (clarsimp)
+         apply fastforce
+    apply fastforce
+   apply (case_tac Q)
+  apply clarsimp
+   apply fastforce
+  apply (case_tac Q)
+  apply clarsimp
+  by fastforce
+
+definition wp_single :: "com \<Rightarrow> com \<Rightarrow> post \<Rightarrow> assn" where
+  "wp_single c1 c2 R = (\<lambda>s. case R of
+      OK Q \<Rightarrow> (\<exists>s'. (c1,sOK s) \<rightarrow> (c2,sOK s') \<and> Q s')
+    | ER Q \<Rightarrow> (\<exists>s'. (c1,sOK s) \<rightarrow> (c2,sER s') \<and> Q s'))"
+
+
+lemma wp_single_ABORT: "wp_single ABORT SKIP R = (case R of
+      OK Q \<Rightarrow> (\<lambda>s. False)
+    | ER Q \<Rightarrow> Q)" 
+  apply (case_tac R)
+   apply clarsimp
+  unfolding wp_single_def apply fastforce
+  apply clarsimp
+  unfolding wp_single_def apply fastforce
+  done
