SIL-Parallel/SIL_Star_Sound.thy
@@ -1,0 +1,112 @@
+subsection \<open>Soundness and Completeness\<close>
+
+theory SIL_Star_Sound
+imports SIL_Star
+begin
+
+subsubsection "Soundness"
+
+lemma sil_while_sound_ok:
+assumes "\<And>n. \<turnstile> \<langle>Q (Suc n)\<rangle> c  \<langle>OK (Q n)\<rangle>"
+      and "\<And>s. Q 0 s \<Longrightarrow> \<not> bval b s"
+      and "\<And>n s. Q (Suc n) s \<Longrightarrow>  bval b s"
+      and "Q n s"
+      and "\<And>n. \<forall>s. Q (Suc n) s \<longrightarrow> (\<exists>t. (c, sOK s) \<rightarrow>* (SKIP, sOK t) \<and> Q n t)"
+    shows "(\<exists>t. (WHILE b DO c, sOK s) \<rightarrow>* (SKIP, sOK t) \<and> Q 0 t)"
+  using assms
+  apply (induct n arbitrary: s)
+   apply (metis While small_step.IfFalse star.simps)
+  by (smt (verit, ccfv_threshold) Small_Step.WhileE Small_Step.post.distinct(1)
+      com.distinct(13) final_def final_iff_SKIP seq_comp_sOK small_step.IfTrue star.step)
+
+lemma sil_while_sound_er:
+  assumes "\<And>n. \<turnstile> \<langle>Q (Suc (Suc n))\<rangle> c \<langle>OK (Q (Suc n))\<rangle>"
+  and "\<turnstile> \<langle>Q 1\<rangle> c \<langle>ER (Q 0)\<rangle>"
+  and "\<And>s. Q 1 s \<Longrightarrow> (\<exists>t. (c, sOK s) \<rightarrow>* (SKIP, sER t) \<and> Q 0 t)"
+  and "\<And>n s. Q (Suc n) s \<Longrightarrow> bval b s"
+  and "Q (Suc m) s"
+  and "\<And>n. \<forall>s. Q (Suc (Suc n)) s \<longrightarrow> (\<exists>t. (c, sOK s) \<rightarrow>* (SKIP, sOK t) \<and> Q (Suc n) t)"
+  shows "\<exists>t. (WHILE b DO c, sOK s) \<rightarrow>* (SKIP, sER t) \<and> Q 0 t"
+  using assms
+  apply (induct m arbitrary: s)
+  apply (smt (verit) One_nat_def Small_Step.IfE Small_Step.WhileE Small_Step.post.distinct(1)
+      com.distinct(13,9) final_def final_iff_SKIP post_state.simps(1) seq_comp_sER star.simps)
+  apply clarsimp
+  sorry
+
+
+
+
+lemma sil_star_sound: 
+  "\<turnstile> \<langle>P\<rangle> c \<langle>R\<rangle>  \<Longrightarrow>  \<Turnstile> \<langle>P\<rangle> c \<langle>R\<rangle>"
+  unfolding SIL_Star_Valid_def
+  apply (induction rule:SIL_Star.induct)
+                      apply fastforce
+                      apply fastforce
+                     apply fastforce
+                    apply fastforce
+                   apply clarsimp
+                   defer
+  apply (case_tac R)
+                    apply clarsimp
+  using seq_comp_sOK apply blast
+                   apply clarsimp
+                   apply (metis seq_comp_sOK)
+                  apply clarsimp
+                  apply (metis seq_comp_sER)
+                 apply (case_tac R)
+  apply clarsimp
+                  apply (metis small_step.IfFalse small_step.IfTrue star.step)
+                 apply (case_tac R)
+                  apply clarsimp
+                 apply clarsimp
+                 apply (metis small_step.IfFalse small_step.IfTrue star.step)
+                apply (case_tac Q)
+                 apply clarsimp
+    defer
+                 apply (case_tac Q)
+                  apply clarsimp
+                 apply clarsimp
+                 defer
+                 apply clarsimp
+                 apply (metis SelectNDN small_step.Abort star.simps)
+                apply clarsimp
+                defer
+                apply clarsimp
+                defer
+  apply fastforce
+               apply fastforce
+              apply (case_tac Q)
+               apply fastforce
+              apply fastforce
+             apply (case_tac Q)
+              apply fastforce
+             apply fastforce
+            defer
+            defer
+            defer
+            defer
+            apply (case_tac Q)
+             apply clarsimp
+             apply (metis ParSkipL star.step)
+            apply clarsimp
+            apply (meson ParSkipL star.step)
+            apply (case_tac Q)
+             apply clarsimp
+             apply (metis ParSkipR star.step)
+            apply clarsimp
+           apply (meson ParSkipR star.step)
+          apply (meson small_step.Abort small_step.AssignNDEmpty star.step star_step1)
+         apply (smt (verit) case_prodD small_step.SelectND star.step)
+        apply (smt (verit, best) case_prod_conv small_step.SelectND star.step)
+       apply (simp add: sil_while_sound_ok)
+      apply (smt (verit, ccfv_threshold) One_nat_def sil_while_sound_er)
+  sledgehammer
+  
+
+
+                
+
+
+
+
